Rules.thy
@@ -35,7 +35,7 @@ inductive rules :: "'b rpred \<Rightarrow> 'b rpred \<Rightarrow> 'b set \<Right
       {(m,m') |m m'. (merge m s, merge m' s) \<in> R},
       {(m,m') |m m'. (merge m s, merge m' s') \<in> G} 
       \<turnstile> {m |m. merge m s \<in> P} {Capture s c} {m |m. merge m s' \<in> Q}" *)
-  | capall[intro]: "R,G \<turnstile> P {c} Q \<Longrightarrow> R,G \<turnstile> P {CaptureAll c} P'"
+  | capall[intro]: "R,G \<turnstile> P {c} Q \<Longrightarrow> stable R P \<Longrightarrow> R,G \<turnstile> P {CaptureAll c} P"
 
 subsection \<open>Properties\<close>
 
@@ -79,13 +79,13 @@ lemma stable_preE:
   assumes "R,G \<turnstile> P {c} Q"
   shows "\<exists>P'. P \<subseteq> P' \<and> stable R P' \<and> R,G \<turnstile> P' {c} Q"
   using assms 
-proof (induct) 
+proof (induct ) 
   case (thread R G P c Q)
   then show ?case by (metis rules.thread)
 next 
   case (par R\<^sub>1 G\<^sub>1 P\<^sub>1 c\<^sub>1 Q\<^sub>1 R\<^sub>2 G\<^sub>2 P\<^sub>2 c\<^sub>2 Q\<^sub>2)
-  obtain P\<^sub>1' where 1: "P\<^sub>1 \<subseteq> P\<^sub>1'" "stable R\<^sub>1 P\<^sub>1'" "R\<^sub>1,G\<^sub>1 \<turnstile> P\<^sub>1' {c\<^sub>1} Q\<^sub>1" using par by auto
-  obtain P\<^sub>2' where 2: "P\<^sub>2 \<subseteq> P\<^sub>2'" "stable R\<^sub>2 P\<^sub>2'" "R\<^sub>2,G\<^sub>2 \<turnstile> P\<^sub>2' {c\<^sub>2} Q\<^sub>2" using par by auto
+  obtain P\<^sub>1' where 1: "P\<^sub>1 \<subseteq> P\<^sub>1'" "stable R\<^sub>1 P\<^sub>1'" "R\<^sub>1,G\<^sub>1 \<turnstile> P\<^sub>1' {c\<^sub>1} Q\<^sub>1" using par(2) by blast
+  obtain P\<^sub>2' where 2: "P\<^sub>2 \<subseteq> P\<^sub>2'" "stable R\<^sub>2 P\<^sub>2'" "R\<^sub>2,G\<^sub>2 \<turnstile> P\<^sub>2' {c\<^sub>2} Q\<^sub>2" using par(4) by blast
   hence "R\<^sub>1 \<inter> R\<^sub>2,G\<^sub>1 \<union> G\<^sub>2 \<turnstile> P\<^sub>1' \<inter> P\<^sub>2' {c\<^sub>1 || c\<^sub>2} Q\<^sub>1 \<inter> Q\<^sub>2" using 1 2 rules.par par(5,6) by simp
   thus ?case using 1 2 stable_conjI by blast
 next
@@ -113,12 +113,6 @@ next
   hence "stable R (\<Inter>s\<in>S. P\<^sub>s s)" by (auto simp: stable_def)
   moreover have "P \<subseteq> (\<Inter>s\<in>S. P\<^sub>s s)" using s by auto
   ultimately show ?case using s seqset.hyps(1) by blast
-next
-  case (capall R G P c Q)
-  then obtain P' where p': "P \<subseteq> P'" "stable R P'" "R,G \<turnstile> P' {c} Q" by blast
-  hence "R,G \<turnstile> P' {CaptureAll c} P'" using rules.capall by blast
-  hence "R,G \<turnstile> P' {CaptureAll c} P" using rules.conseq p'(1) by try0
-  then show ?case using rules.capall 
 qed blast+
 
 lemma false_seqI [intro]:
@@ -134,6 +128,9 @@ proof (induct c)
 next
   case (SeqChoice x)
   thus ?case by (intro ballI seqset false_seqI) auto
+next         
+  case (Capture x1 c)
+  then show ?case sorry
 qed auto
 
 lemma seq_rot:
